ulib/FStar.Tactics.Typeclasses.fst
@@ -87,7 +87,7 @@ let mk_class (nm:string) : Tac decls =
     (* dump ("got it, ty = " ^ term_to_string ty); *)
     let ctor_name = last name in
     // Must have a single constructor
-    guard (List.length ctors = 1);
+    guard (List.Tot.Base.length ctors = 1);
     let [ctor] = ctors in
     let r = lookup_typ (top_env ()) ctor in
     guard (Some? r);
@@ -102,9 +102,9 @@ let mk_class (nm:string) : Tac decls =
     let C_Total cod _ = r in (* must be total *)
     (* The constructor of course takes the parameters of the record
      * as arguments, but we should ignore them here *)
-    let ps, bs = List.Tot.splitAt (List.length params) bs in
+    let ps, bs = List.Tot.Base.splitAt (List.Tot.Base.length params) bs in
 
-    (* print ("n_univs = " ^ string_of_int (List.length us)); *)
+    (* print ("n_univs = " ^ string_of_int (List.Tot.Base.length us)); *)
 
     let base : string = "__proj__Mk" ^ ctor_name ^ "__item__" in
 
@@ -132,7 +132,7 @@ let mk_class (nm:string) : Tac decls =
                   //dump ("proj_ty = " ^ term_to_string proj_ty);
                   let ty =
                     let bs, cod = collect_arr_bs proj_ty in
-                    let ps, bs = List.Tot.splitAt (List.length params) bs in
+                    let ps, bs = List.Tot.Base.splitAt (List.Tot.Base.length params) bs in
                     match bs with
                     | [] -> fail "mk_class: impossible, no binders"
                     | b1::bs' ->
